src/Init/Data/Array/Subarray.lean
@@ -48,7 +48,7 @@ instance : GetElem (Subarray α) Nat α fun xs i => i < xs.size where
   getElem xs i h := xs.get ⟨i, h⟩
 
 @[inline] def getD (s : Subarray α) (i : Nat) (v₀ : α) : α :=
-  if h : i < s.size then s.get ⟨i, h⟩ else v₀
+  if h : i < s.size then s[i] else v₀
 
 abbrev get! [Inhabited α] (s : Subarray α) (i : Nat) : α :=
   getD s i default
