src/Init/GetElem.lean
@@ -224,7 +224,7 @@ end List
 namespace Array
 
 instance : GetElem (Array α) Nat α fun xs i => i < xs.size where
-  getElem xs i h := xs.get ⟨i, h⟩
+  getElem xs i h := xs.get i h
 
 end Array
 
