src/Lean/Data/PersistentHashMap.lean
@@ -84,11 +84,10 @@ private theorem size_push {ks : Array α} {vs : Array β} (h : ks.size = vs.size
 partial def insertAtCollisionNodeAux [BEq α] : CollisionNode α β → Nat → α → β → CollisionNode α β
   | n@⟨Node.collision keys vals heq, _⟩, i, k, v =>
     if h : i < keys.size then
-      let idx : Fin keys.size := ⟨i, h⟩;
-      let k' := keys.get idx;
+      let k' := keys[i];
       if k == k' then
          let j : Fin vals.size := ⟨i, by rw [←heq]; assumption⟩
-         ⟨Node.collision (keys.set idx k) (vals.set j v) (size_set heq idx j k v), IsCollisionNode.mk _ _ _⟩
+         ⟨Node.collision (keys.set i k) (vals.set j v) (size_set heq ⟨i, h⟩ j k v), IsCollisionNode.mk _ _ _⟩
       else insertAtCollisionNodeAux n (i+1) k v
     else
       ⟨Node.collision (keys.push k) (vals.push v) (size_push heq k v), IsCollisionNode.mk _ _ _⟩
