src/Lean/Meta/Match/Match.lean
@@ -546,7 +546,7 @@ private def processValue (p : Problem) : MetaM (Array Problem) := do
   subgoals.mapIdxM fun i subgoal => do
     trace[Meta.Match.match] "processValue subgoal\n{MessageData.ofGoal subgoal.mvarId}"
     if h : i < values.size then
-      let value := values.get ⟨i, h⟩
+      let value := values[i]
       -- (x = value) branch
       let subst := subgoal.subst
       trace[Meta.Match.match] "processValue subst: {subst.map.toList.map fun p => mkFVar p.1}, {subst.map.toList.map fun p => p.2}"
