src/Lean/Meta/WHNF.lean
@@ -184,7 +184,7 @@ private def cleanupNatOffsetMajor (e : Expr) : MetaM Expr := do
 private def reduceRec (recVal : RecursorVal) (recLvls : List Level) (recArgs : Array Expr) (failK : Unit → MetaM α) (successK : Expr → MetaM α) : MetaM α :=
   let majorIdx := recVal.getMajorIdx
   if h : majorIdx < recArgs.size then do
-    let major := recArgs.get ⟨majorIdx, h⟩
+    let major := recArgs[majorIdx]
     let mut major ← if isWFRec recVal.name && (← getTransparency) == .default then
       -- If recursor is `Acc.rec` or `WellFounded.rec` and transparency is default,
       -- then we bump transparency to .all to make sure we can unfold defs defined by WellFounded recursion.
@@ -226,7 +226,7 @@ private def reduceRec (recVal : RecursorVal) (recLvls : List Level) (recArgs : A
 private def reduceQuotRec (recVal  : QuotVal) (recArgs : Array Expr) (failK : Unit → MetaM α) (successK : Expr → MetaM α) : MetaM α :=
   let process (majorPos argPos : Nat) : MetaM α :=
     if h : majorPos < recArgs.size then do
-      let major := recArgs.get ⟨majorPos, h⟩
+      let major := recArgs[majorPos]
       let major ← whnf major
       match major with
       | Expr.app (Expr.app (Expr.app (Expr.const majorFn _) _) _) majorArg => do
@@ -255,7 +255,7 @@ mutual
     else do
       let majorIdx := recVal.getMajorIdx
       if h : majorIdx < recArgs.size then do
-        let major := recArgs.get ⟨majorIdx, h⟩
+        let major := recArgs[majorIdx]
         let major ← whnf major
         getStuckMVar? major
       else
@@ -264,7 +264,7 @@ mutual
   private partial def isQuotRecStuck? (recVal : QuotVal) (recArgs : Array Expr) : MetaM (Option MVarId) :=
     let process? (majorPos : Nat) : MetaM (Option MVarId) :=
       if h : majorPos < recArgs.size then do
-        let major := recArgs.get ⟨majorPos, h⟩
+        let major := recArgs[majorPos]
         let major ← whnf major
         getStuckMVar? major
       else
